WIP: Lemmas about contexts (too technical!). Correct the statement of Sat.applDual

Hybrid/Language/Context.lean
@@ -67,4 +67,55 @@ def FormL.Context.subst {φ : Form sig s}
 
 notation:max C:49 "[" φ:50 "]" => FormL.Context.subst C φ
 
-def idk {φ χ : Form symbs s} {ψ : FormL symbs sorts} (C : φ.Context ψ) : χ.Context C[χ] := sorry
+/-
+def FormL.Context.index {φ : Form symbs s} {ψ : FormL symbs sorts}: φ.Context ψ → Fin (sorts.length)
+  | .refl => Fin.mk 0 (by simp only [List.length_singleton, Nat.lt_succ_self])
+  | .head => Fin.mk 0 (by simp only [List.length_cons, Nat.lt_add_left_iff_pos, Nat.zero_lt_succ])
+  | @FormL.Context.tail _ _ _ _ _ sorts' ψ' _ _ ctx' => Fin.mk (1 + ctx'.index.val) (by
+          have := ctx'.index.isLt
+          simp only [List.length_cons, Nat.lt_succ] at this ⊢
+          rw [Nat.add_comm]
+          exact Nat.add_le_add_right this 1
+      )
+
+def FormL.Context.from_index {φ : Form symbs s} {ψ : FormL symbs sorts} : Fin (sorts.length) → Option (φ.Context ψ)
+  | ⟨0, h⟩ => sorry
+  | ⟨n+1, h⟩ => sorry
+-/
+
+def FormL.Context.index {φ : Form symbs s} {ψ : FormL symbs sorts}: φ.Context ψ → Nat
+  | .refl => 0
+  | .head => 0
+  | .tail ctx' => 1 + ctx'.index
+
+def FormL.Context.from_index {φ : Form symbs s} {ψ : FormL symbs sorts} : Nat → Option (φ.Context ψ)
+  | 0   => sorry
+  | n+1 => sorry
+
+def FormL.Context.iso {φ : Form symbs s} {ψ : Form symbs s'} {χ τ : FormL symbs sorts} (C₁ : φ.Context χ) (C₂ : ψ.Context τ) : Prop :=
+  match C₁ with
+  | .refl =>
+      match C₂ with
+      | .refl => True
+  | .head =>
+      match C₂ with
+      | .head => True
+      | _ => False
+  | .tail ctx =>
+      match C₂ with
+      | .tail ctx' => ctx.iso ctx'
+      | _ => False
+
+lemma FormL.Context.iso_trans {φ : Form symbs s} {ψ : Form symbs s'} {χ : Form symbs s''} {a b c : FormL symbs sorts} {C₁ : φ.Context a} {C₂ : ψ.Context b} {C₃ : χ.Context c} : C₁.iso C₂ → C₁.iso C₃ → C₂.iso C₃ := sorry
+
+lemma FormL.Context.if_iso {φ ψ : Form symbs s} {τ : FormL symbs sorts} (C₁ : φ.Context τ) (C₂ : ψ.Context τ) (h : C₁.iso C₂) : φ = ψ := sorry
+
+lemma FormL.Context.if_iso_sorts {φ : Form symbs s} {ψ : Form symbs s'} {τ : FormL symbs sorts} (C₁ : φ.Context τ) (C₂ : ψ.Context τ) (h : C₁.iso C₂) : s = s' := sorry
+
+lemma FormL.Context.iso_subst {φ ψ χ : Form symbs s} {τ : FormL symbs sorts} {C₁ : φ.Context τ} {C₂ : ψ.Context C₁[χ]} (h : C₁.iso C₂) : ψ = χ := sorry
+
+def FormL.Context.subst_iso {φ ψ : Form symbs s} {χ : FormL symbs sorts} {C₁ : φ.Context χ} (C₂ : ψ.Context C₁[ψ]) (h : C₁.iso C₂) : (τ : Form symbs s) → Σ' C₃ : τ.Context C₁[τ], C₂.iso C₃ := sorry
+
+def FormL.Context.subst_not_iso {φ ψ χ : Form symbs s} {τ : FormL symbs sorts} {C₁ : φ.Context τ} (C₂ : ψ.Context C₁[χ]) (h : ¬C₁.iso C₂) : (δ : Form symbs s) → Σ' C₃ : ψ.Context C₁[δ], C₂.iso C₃ := sorry
+
+def FormL.Context.subst_not_iso' {φ : Form symbs s} {ψ : Form symbs s'} {τ : FormL symbs sorts} {C₁ : φ.Context τ} (C₂ : ψ.Context τ) (h : ¬C₁.iso C₂) : (δ : Form symbs s) → Σ' C₃ : ψ.Context C₁[δ], C₂.iso C₃ := sorry
